src/Specific/IntegrationTestMontgomeryP256_128_SubDisplay.v
@@ -1,0 +1,4 @@
+Require Import Crypto.Specific.IntegrationTestMontgomeryP256_128_Sub.
+Require Import Crypto.Specific.IntegrationTestDisplayCommon.
+
+Check display sub.
