src/Specific/NISTP256/AMD64/IntegrationTestMontgomeryP256_SubDisplay.v
@@ -1,0 +1,4 @@
+Require Import Crypto.Specific.NISTP256.AMD64.IntegrationTestMontgomeryP256_Sub.
+Require Import Crypto.Specific.IntegrationTestDisplayCommon.
+
+Check display sub.
